src/proof/kubernetes_model/inv.v
@@ -11,7 +11,7 @@ Section spec.
 Context `{hG: !heapGS Σ} {go_ctx: GoContext}.
 Context `{!kviewG Σ}.
 
-Definition obj_parent_ref obj: option (KKey.t * types.UID.t) :=
+Definition obj_parent_ref obj : option (KKey.t * types.UID.t) :=
   match (KObjectV.objectmeta obj).(ObjectMetaV.OwnerReferences') with
   | Some orefs => match list_find (λ oref, oref.(OwnerReferenceV.Controller') = Some true) orefs with
     | Some (_, oref) => Some (
@@ -27,7 +27,7 @@ Definition obj_parent_ref obj: option (KKey.t * types.UID.t) :=
   | None => None
   end.
 
-Definition obj_ref k obj: KKey.t * types.UID.t :=
+Definition obj_ref k obj : KKey.t * types.UID.t :=
   (k, (KObjectV.objectmeta obj).(ObjectMetaV.UID')).
 
 Context `{!cviewG KKey.t (KKey.t * types.UID.t) KObjectV.t obj_parent_ref obj_ref Σ}.
@@ -40,45 +40,49 @@ Record KubernetesGname := mk_γk {
   γ_tombstone : gname;
 }.
 
-Definition own_kview_auth γ state used_uids: iProp Σ :=
-  kview.own_auth γ.(γ_state) state used_uids.
+Definition own_kview_auth γ state used_uid : iProp Σ :=
+  kview.own_auth γ.(γ_state) state used_uid.
 
-Definition own_meta_frag γ k uid dq m: iProp Σ :=
+Definition own_meta_frag γ k uid dq m : iProp Σ :=
   kview.own_meta_frag γ.(γ_state) k uid dq m.
 
-Definition own_spec_frag γ k uid dq sp: iProp Σ :=
+Definition own_spec_frag γ k uid dq sp : iProp Σ :=
   kview.own_spec_frag γ.(γ_state) k uid dq sp.
 
-Definition own_status_frag γ k uid dq st: iProp Σ :=
+Definition own_status_frag γ k uid dq st : iProp Σ :=
   kview.own_status_frag γ.(γ_state) k uid dq st.
 
-Definition own_children_auth γ state used_references: iProp Σ :=
+Definition own_children_auth γ state used_reference : iProp Σ :=
   cview.own_auth KKey.t (KKey.t * types.UID.t) KObjectV.t obj_parent_ref obj_ref
-  γ.(γ_children) state used_references.
+  γ.(γ_children) state used_reference.
 
-Definition own_children_frag γ key uid dq keys: iProp Σ :=
+Definition own_children_frag γ key uid dq keys : iProp Σ :=
   cview.own_frag KKey.t (KKey.t * types.UID.t) KObjectV.t obj_parent_ref obj_ref
   γ.(γ_children) (key, uid) dq keys.
 
-Definition own_tombstone_auth γ tombed_uids: iProp Σ :=
-  mono_gset.own_auth types.UID.t γ.(γ_tombstone) tombed_uids.
+Definition own_tombstone_auth γ tombed_uid : iProp Σ :=
+  mono_gset.own_auth types.UID.t γ.(γ_tombstone) tombed_uid.
 
-Definition own_tombstone_frag γ tombed_uid: iProp Σ :=
+Definition own_tombstone_frag γ tombed_uid : iProp Σ :=
   mono_gset.own_frag types.UID.t γ.(γ_tombstone) tombed_uid.
 
-Definition kubernetes_inv γ l: iProp Σ :=
-  ∃ (phys_state_l: loc) (rvc: w64) (phys_state: gmap KKey.t interface.t)
-    (abs_state: gmap KKey.t KObjectV.t) (used_uids: gset types.UID.t)
-    (tombed_uids: gset types.UID.t) (used_references: gset (KKey.t * types.UID.t)),
+Definition kubernetes_inv γ l : iProp Σ :=
+  ∃ (phys_state_l: loc) (phys_used_uid_l: loc) (rvc: w64)
+    (phys_state: gmap KKey.t interface.t) (phys_used_uid : gmap types.UID.t unit)
+    (abs_state: gmap KKey.t KObjectV.t) (used_uid: gset types.UID.t) (tombed_uid: gset types.UID.t)
+    (used_reference: gset (KKey.t * types.UID.t)),
     "Hstate_m_addr" ∷ l ↦s[apimodel.State :: "m"] phys_state_l ∗
+    "Hstate_used_uid_addr" ∷ l ↦s[apimodel.State :: "usedUID"] phys_used_uid_l ∗
     "Hstate_rvc_addr" ∷ l ↦s[apimodel.State :: "resourceVersionCounter"] rvc ∗
     "Hown_phys" ∷ phys_state_l ↦$ phys_state ∗
-    "Hown_abs" ∷ own_kview_auth γ abs_state used_uids ∗
-    "Hown_children" ∷ own_children_auth γ abs_state used_references ∗
-    "Hown_tombstone" ∷ own_tombstone_auth γ tombed_uids ∗
+    "Hown_used_uid" ∷ phys_used_uid_l ↦$ phys_used_uid ∗
+    "Hown_abs" ∷ own_kview_auth γ abs_state used_uid ∗
+    "Hown_children" ∷ own_children_auth γ abs_state used_reference ∗
+    "Hown_tombstone" ∷ own_tombstone_auth γ tombed_uid ∗
     "Hphys_abs_rep" ∷ ([∗ map] i; obj ∈ phys_state; abs_state, KObjectV.deepown_i i obj 1) ∗
-    "%Hused_uids_eq" ∷ ⌜ used_uids = (set_map (λ v, snd v) used_references) ⌝ ∗
-    "%Htombed_uids_eq" ∷ ⌜ tombed_uids = used_uids ∖ map_to_set (λ _ obj, (KObjectV.objectmeta obj).(ObjectMetaV.UID')) abs_state ⌝.
+    "%Hused_uid_eq_dom_phys_used_uid" ∷ ⌜ used_uid = dom phys_used_uid ⌝ ∗ 
+    "%Hused_uid_eq_set_map_used_reference" ∷ ⌜ used_uid = (set_map (λ v, snd v) used_reference) ⌝ ∗
+    "%Htombed_uid_eq_used_uid_sub" ∷ ⌜ tombed_uid = used_uid ∖ map_to_set (λ _ obj, (KObjectV.objectmeta obj).(ObjectMetaV.UID')) abs_state ⌝.
 
 Definition is_kubernetes γ l : iProp Σ :=
   ∃ (mu_l: loc),
